ProofLibrary/List.lean
@@ -5,16 +5,6 @@ section
   -- copied from mathlib
   theorem Nat.min_succ_succ (x y : Nat) : min (succ x) (succ y) = succ (min x y) := by
     simp [Nat.min_def, Nat.succ_le_succ_iff]; split <;> rfl
-
-  theorem List.take_succ_cons : (a :: as).take (i + 1) = a :: as.take i := rfl
-  theorem List.length_take : ∀ (i : Nat) (l : List α), length (take i l) = min i (length l)
-    | 0, l => by simp [List.length, Nat.zero_min]
-    | Nat.succ n, [] => by simp [List.length, Nat.min_zero]
-    | Nat.succ n, _ :: l => by simp [Nat.min_succ_succ, Nat.add_one, length_take, take_succ_cons]
-  theorem List.length_take_le (n) (l : List α) : length (take n l) ≤ n := by simp [List.length_take, Nat.min_le_left]
-
-  theorem List.get_map (f : α → β) {l n} : get (map f l) n = f (get l ⟨n, length_map l f ▸ n.2⟩) := 
-    Option.some.inj <| by rw [← get?_eq_get, get?_map, get?_eq_get]; rfl
 end 
 
 namespace List
@@ -34,22 +24,22 @@ namespace List
         | inl h_in_head => left; unfold Set.element at h_in_head; rw [h_in_head]
         | inr h_in_tail => right; rw [ih]; exact h_in_tail
 
-  theorem listToSetElementAlsoListElement [BEq α] [LawfulBEq α] (L : List α) (e : α) : e ∈ L.toSet -> L.elem e := by 
+  theorem listToSetElementAlsoListElement [BEq α] [LawfulBEq α] (L : List α) (e : α) : e ∈ L.toSet -> e ∈ L := by 
     induction L with 
       | nil => intros; contradiction
       | cons head tail ih => intro h; simp [Set.element, toSet] at h; cases h with 
-        | inl left => simp [Set.element] at left; simp [left, elem]
-        | inr right => simp [elem]; cases e == head with | true => rfl | false => exact (ih right) 
+        | inl left => simp [Set.element] at left; simp [left]
+        | inr right => simp; cases eq : e == head with | true => apply Or.inl; apply LawfulBEq.eq_of_beq; exact eq | false => apply Or.inr; exact (ih right) 
 
-  theorem listElementAlsoToSetElement [BEq α] [LawfulBEq α] (L : List α) (e : α) : L.elem e -> e ∈ L.toSet := by 
+  theorem listElementAlsoToSetElement (L : List α) (e : α) : e ∈ L -> e ∈ L.toSet := by 
     induction L with  
       | nil => intros; contradiction 
       | cons head tail ih => 
-        unfold elem; unfold Set.element; unfold toSet; split 
-        case h_1 _ h => intros; apply Or.inl; unfold Set.element; apply LawfulBEq.eq_of_beq; exact h
-        case h_2 => intro h; apply Or.inr; apply ih; apply h
+        simp; unfold Set.element; unfold toSet; intro h_inList; cases h_inList with 
+        | inl hl => apply Or.inl; unfold Set.element; exact hl
+        | inr hr => apply Or.inr; apply ih; apply hr
 
-  theorem listElementIffToSetElement [BEq α] [LawfulBEq α] (L : List α) (e : α) : L.elem e ↔ e ∈ L.toSet := by 
+  theorem listElementIffToSetElement [BEq α] [LawfulBEq α] (L : List α) (e : α) : e ∈ L ↔ e ∈ L.toSet := by 
     constructor; apply listElementAlsoToSetElement; apply listToSetElementAlsoListElement
 
   theorem listGetInToSet (L : List α) (indexFin : Fin L.length) : L.get indexFin ∈ L.toSet := by
@@ -71,19 +61,20 @@ namespace List
           | inl eIsA => apply Or.inl; rw [eIsA]
           | inr eInAs => apply Or.inr; apply mappedElemInMappedList; exact eInAs
 
-  theorem exElemInMappedListMeansOriginalElemExistsThatMapsToIt [BEq α] [BEq β] [LawfulBEq α] [LawfulBEq β] (L : List α) (f : α -> β) (e : β): List.elem e (L.map f) -> (∃ e', List.elem e' L ∧ e = f e') := by 
-    induction L with 
+  theorem exElemInMappedListMeansOriginalElemExistsThatMapsToIt (L : List α) (f : α -> β) (e : β): e ∈ (L.map f) -> (∃ e', e' ∈ L ∧ e = f e') := by 
+    cases L with 
     | nil => intros; contradiction
-    | cons head tail ih =>
+    | cons head tail =>
       intro he 
-      simp [elem, map] at he
-      split at he
-      . exists head; constructor; simp [elem]; apply LawfulBEq.eq_of_beq; assumption
-      . cases ih he with | intro e' he' => 
-        exists e'
-        constructor 
-        . unfold elem; split; rfl; exact he'.left
-        . exact he'.right
+      simp [map] at he
+      cases he with 
+      | inl _ => exists head; constructor; simp; assumption
+      | inr hr =>
+        cases hr with | intro e' he' => 
+          exists e'
+          constructor 
+          . simp; right; exact he'.left
+          . apply Eq.symm; exact he'.right
 
   theorem combine_nested_map (L : List α) (f : α -> β) (g : β -> γ) : List.map g (List.map f L) = List.map (g ∘ f) L := by
     induction L 
@@ -176,14 +167,14 @@ namespace List
   def enum_with_lt (l : List α) : List ((Fin l.length) × α) :=
     l.enum_with_lt_from 0 l.length (by simp)
 
-  def idx_of_with_count [DecidableEq α] (l : List α) (e : α) (e_in_l : l.elem e) (c : Nat) : Fin (c + l.length) :=
+  def idx_of_with_count [DecidableEq α] (l : List α) (e : α) (e_in_l : e ∈ l) (c : Nat) : Fin (c + l.length) :=
     match l with 
       | nil => by contradiction
       | cons h tail => if eq : e == h then ⟨c, by simp [length]; rw [← Nat.add_zero c]; apply (Nat.add_lt_add_left (by show 0 < (tail.length + 1); apply Nat.zero_lt_of_ne_zero; apply Nat.succ_ne_zero) c)⟩ else 
-        let res := tail.idx_of_with_count e (by unfold elem at e_in_l; simp [eq] at e_in_l; exact e_in_l) (c + 1) 
+        let res := tail.idx_of_with_count e (by cases e_in_l; simp at eq; assumption) (c + 1) 
         ⟨res.val, by simp [length]; rw [@Nat.add_comm tail.length 1, ← Nat.add_assoc]; exact res.isLt⟩
 
-  theorem idx_of_with_count_succ [DecidableEq α] (l : List α) (e : α) (e_in_l : l.elem e) (c : Nat) : (idx_of_with_count l e e_in_l (c + 1)).val = (idx_of_with_count l e e_in_l c).val + 1 := by
+  theorem idx_of_with_count_succ [DecidableEq α] (l : List α) (e : α) (e_in_l : e ∈ l) (c : Nat) : (idx_of_with_count l e e_in_l (c + 1)).val = (idx_of_with_count l e e_in_l c).val + 1 := by
     induction l generalizing c with 
     | nil => contradiction
     | cons b bs ih =>
@@ -192,30 +183,27 @@ namespace List
       case pos hl => simp [hl]
       case neg hr => simp [hr]; apply ih
 
-  def idx_of [DecidableEq α] (l : List α) (e : α) (e_in_l : l.elem e) : Fin l.length :=
+  def idx_of [DecidableEq α] (l : List α) (e : α) (e_in_l : e ∈ l) : Fin l.length :=
     let tmp_fin := l.idx_of_with_count e e_in_l 0
     have tmp_fin_isLt := tmp_fin.isLt
     ⟨tmp_fin.val, by simp at tmp_fin_isLt; exact tmp_fin_isLt⟩
 
   theorem get_prepend_succ [DecidableEq α] (l : List α) (a : α) (i : Fin l.length) (j : Fin (a::l).length) (h : j = Fin.succ i) : l.get i = (a::l).get j := by rw [h]; simp [get]
 
-  theorem idx_of_prepend_succ [DecidableEq α] (l : List α) (e a : α) (e_in_l : l.elem e) (h : e ≠ a) : ((a::l).idx_of e (by unfold elem; split <;> trivial)) = Fin.succ (l.idx_of e e_in_l) := by 
+  theorem idx_of_prepend_succ [DecidableEq α] (l : List α) (e a : α) (e_in_l : e ∈ l) (h : e ≠ a) : ((a::l).idx_of e (by right; trivial)) = Fin.succ (l.idx_of e e_in_l) := by 
     simp [idx_of, idx_of_with_count, h, Fin.succ]
     apply idx_of_with_count_succ
 
-  theorem idx_of_get [DecidableEq α] (l : List α) (e : α) (e_in_l : l.elem e) (isLt : (l.idx_of e e_in_l < l.length)) : e = l.get ⟨(l.idx_of e e_in_l).val, isLt⟩ := by 
+  theorem idx_of_get [DecidableEq α] (l : List α) (e : α) (e_in_l : e ∈ l) (isLt : (l.idx_of e e_in_l < l.length)) : e = l.get ⟨(l.idx_of e e_in_l).val, isLt⟩ := by 
     induction l with 
     | nil => contradiction
     | cons a as ih =>
       by_cases h : e = a
       . simp [get, h, idx_of, idx_of_with_count]
-      . have e_in_as : as.elem e := by 
-          unfold elem at e_in_l
-          split at e_in_l 
-          case h_1 heq => 
-            have : e = a := LawfulBEq.eq_of_beq heq
-            contradiction
-          case h_2 => trivial
+      . have e_in_as : e ∈ as := by 
+          cases e_in_l 
+          . contradiction
+          . trivial
         have isLt_as : (as.idx_of e e_in_as).val < as.length := by 
           exact (as.idx_of e e_in_as).isLt
         have ih_plugged_in := ih e_in_as isLt_as    
@@ -223,7 +211,7 @@ namespace List
         exact ih_plugged_in
         rw [get_prepend_succ as a (as.idx_of e e_in_as) ((a::as).idx_of e e_in_l) (idx_of_prepend_succ as e a e_in_as h)]
 
-  theorem idx_of_with_count_eq_of_list_eq [DecidableEq α] (l l' : List α) (h : l = l') (e : α) (he : l.elem e) : ∀ c, (l.idx_of_with_count e he c).val = (l'.idx_of_with_count e (by rw [← h]; exact he) c).val := by 
+  theorem idx_of_with_count_eq_of_list_eq [DecidableEq α] (l l' : List α) (h : l = l') (e : α) (he : e ∈ l) : ∀ c, (l.idx_of_with_count e he c).val = (l'.idx_of_with_count e (by rw [← h]; exact he) c).val := by 
     cases l with 
     | nil => cases l'; simp; contradiction
     | cons head tail => cases l' with 
@@ -233,22 +221,22 @@ namespace List
         have tails_eq : tail = tail' := by injection h
         simp [idx_of_with_count] 
         split
-        case inl he => simp [he, heads_eq]
-        case inr he => simp [heads_eq] at he; simp [he]; intro c; apply idx_of_with_count_eq_of_list_eq; apply tails_eq
+        case isTrue he => simp [he, heads_eq]
+        case isFalse he => simp [heads_eq] at he; simp [he]; intro c; apply idx_of_with_count_eq_of_list_eq; apply tails_eq
 
-  theorem idx_of_eq_of_list_eq [DecidableEq α] (l l' : List α) (h : l = l') (e : α) (he : l.elem e) : (l.idx_of e he).val = (l'.idx_of e (by rw [← h]; exact he)).val := by 
+  theorem idx_of_eq_of_list_eq [DecidableEq α] (l l' : List α) (h : l = l') (e : α) (he : e ∈ l) : (l.idx_of e he).val = (l'.idx_of e (by rw [← h]; exact he)).val := by 
     apply idx_of_with_count_eq_of_list_eq
     apply h
 
-  theorem idx_of_with_count_eq_under_map [DecidableEq α] [DecidableEq β] (l : List α) (e : α) (he : l.elem e) (f : α -> β) (hf : ∀ e', e' ∈ l.toSet ∧ f e = f e' -> e = e') : ∀ c, (l.idx_of_with_count e he c).val = ((l.map f).idx_of_with_count (f e) (by apply listToSetElementAlsoListElement; apply mappedElemInMappedList; apply listElementAlsoToSetElement; exact he) c).val := by
+  theorem idx_of_with_count_eq_under_map [DecidableEq α] [DecidableEq β] (l : List α) (e : α) (he : e ∈ l) (f : α -> β) (hf : ∀ e', e' ∈ l.toSet ∧ f e = f e' -> e = e') : ∀ c, (l.idx_of_with_count e he c).val = ((l.map f).idx_of_with_count (f e) (by apply listToSetElementAlsoListElement; apply mappedElemInMappedList; apply listElementAlsoToSetElement; exact he) c).val := by
     induction l with 
     | nil => contradiction 
     | cons head tail ih => 
       intro c 
       simp [idx_of_with_count]
       split 
-      case inl he => simp [he]
-      case inr he => 
+      case isTrue he => simp [he]
+      case isFalse he => 
         have : ¬ f e = f head := by 
           intro hcontra; 
           have : e = head := by apply hf; constructor; unfold toSet; apply Or.inl; rfl; apply hcontra
@@ -262,24 +250,13 @@ namespace List
         apply e'InTail
         apply feEqfe'
 
-  theorem idx_of_eq_under_map [DecidableEq α] [DecidableEq β] (l : List α) (e : α) (he : l.elem e) (f : α -> β) (hf : ∀ e', e' ∈ l.toSet ∧ f e = f e' -> e = e') : (l.idx_of e he).val = ((l.map f).idx_of (f e) (by apply listToSetElementAlsoListElement; apply mappedElemInMappedList; apply listElementAlsoToSetElement; exact he)).val := by
+  theorem idx_of_eq_under_map [DecidableEq α] [DecidableEq β] (l : List α) (e : α) (he : e ∈ l) (f : α -> β) (hf : ∀ e', e' ∈ l.toSet ∧ f e = f e' -> e = e') : (l.idx_of e he).val = ((l.map f).idx_of (f e) (by apply listToSetElementAlsoListElement; apply mappedElemInMappedList; apply listElementAlsoToSetElement; exact he)).val := by
     apply idx_of_with_count_eq_under_map 
     apply hf
 
-  theorem length_enum_from (l : List α) (n m : Nat): (l.enumFrom n).length = (l.enumFrom m).length := by 
-    induction l generalizing n m with 
-    | nil => simp [enumFrom]
-    | cons a as ih => unfold enumFrom; unfold length; simp; apply ih
+  theorem length_enum_from' (l : List α) (n : Nat) : (l.enumFrom n).length = l.length := by simp
 
-  theorem length_enum_from' (l : List α) (n : Nat) : (l.enumFrom n).length = l.length := by 
-    induction l generalizing n with
-    | nil => simp [enumFrom]
-    | cons a as ih => unfold enumFrom; unfold length; simp; apply ih
-
-  theorem length_enum (l : List α) : l.enum.length = l.length := by 
-    induction l with 
-    | nil => simp [enum, enumFrom]
-    | cons a as ih => unfold enum at *; unfold enumFrom; unfold length; simp; rw [← ih]; apply length_enum_from
+  theorem length_enum (l : List α) : l.enum.length = l.length := by simp
 
   theorem get_enum_from (l : List α) (n : Nat) (i : Fin l.length) : (l.enumFrom n).get ⟨i.val, (by rw [l.length_enum_from' n]; exact i.isLt)⟩ = (n + i.val, l.get i) := by 
     rw [← Option.someInj, ← get?_eq_get]
@@ -332,10 +309,7 @@ namespace List
     apply map_eq_map_if_functions_eq 
     apply map_eq_map_then_functions_eq
 
-  theorem neg_all_of_any_neg (l : List α) (p : α -> Bool) : l.any (fun a => ¬p a) -> ¬l.all p := by 
-    simp
-    intro x _ _
-    exists x 
+  theorem neg_all_of_any_neg (l : List α) (p : α -> Bool) : l.any (fun a => ¬p a) -> ¬l.all p := by simp
 
   theorem any_of_exists (l : List α) (p : α -> Bool) : (∃ a, a ∈ l.toSet ∧ p a) -> l.any p = true := by 
     simp
@@ -359,52 +333,45 @@ namespace List
   theorem existsIndexIffInToSet [DecidableEq α] (L : List α) (e : α) : (∃ i, e = L.get i) ↔ e ∈ L.toSet := by 
     constructor; apply existsIndexMeansInToSet; apply inToSetMeansExistsIndex
 
-  theorem elemFilterAlsoElemList [BEq α] (L : List α) (f : α -> Bool) : ∀ e, (L.filter f).elem e -> L.elem e := by 
+  theorem elemFilterAlsoElemList (L : List α) (f : α -> Bool) : ∀ e, e ∈ (L.filter f) -> e ∈ L := by 
     induction L with 
     | nil => intros; contradiction
     | cons head tail ih => 
       unfold filter
       split
-      . intro e; unfold elem; split; trivial; apply ih
-      . intros; unfold elem; split; rfl; apply ih; assumption
+      . intro e; intro h; cases h; left; right; apply ih; assumption
+      . intros; right; apply ih; assumption
 
-  theorem elemConcatIffElemOfOne [BEq α] (L L' : List α) : ∀ e, List.elem e (L ++ L') ↔ L.elem e ∨ L'.elem e := by 
-    induction L with 
-    | nil => simp
-    | cons head tail ih => 
-      intro e
-      cases (Decidable.em (e == head)) with 
-      | inl hl => simp [elem, hl]
-      | inr hr => simp [elem, hr]; apply ih
+  theorem elemConcatIffElemOfOne (L L' : List α) : ∀ e, e ∈ (L ++ L') ↔ e ∈ L ∨ e ∈ L' := by simp
 
   def flatten (L : List (List α)) : List α := L.foldl (fun acc L' => acc ++ L') (List.nil)
 
-  theorem elemFlattenAlsoElemSomeListHelper [BEq α] [LawfulBEq α] (L : List (List α)) : ∀ e L', ¬ L'.elem e ∧ (L.foldl (fun acc L'' => acc ++ L'') L').elem e -> ∃ L'', L.elem L'' ∧ L''.elem e := by 
+  theorem elemFlattenAlsoElemSomeListHelper [BEq α] [LawfulBEq α] (L : List (List α)) : ∀ e (L' : List _), ¬e ∈ L' ∧ e ∈ (L.foldl (fun acc L'' => acc ++ L'') L') -> ∃ L'', L'' ∈ L ∧ e ∈ L'' := by 
     induction L with 
     | nil => intro _ _ ⟨not_elem, elem_flatten⟩; contradiction
     | cons head tail ih => 
       intro e L' he
-      simp [foldl] at he
+      simp only [foldl] at he
 
-      cases Decidable.em (head.elem e) with
+      cases Decidable.em (e ∈ head) with
       | inl e_in_head => exists head; constructor; simp [elem]; exact e_in_head
       | inr not_e_in_head => 
         have ex_l_in_tail := ih e (L' ++ head) (by 
           constructor
-          . rw [elemConcatIffElemOfOne]; intro hcontra; cases hcontra with | inl hl => rw [he.left] at hl; contradiction | inr hr => contradiction 
+          . rw [elemConcatIffElemOfOne]; intro hcontra; cases hcontra with | inl hl => apply he.left; exact hl | inr hr => contradiction 
           . exact he.right
         )
         cases ex_l_in_tail with | intro l hl =>
           exists l 
           constructor 
-          . unfold elem; split; rfl; exact hl.left
+          . right; exact hl.left
           . exact hl.right
 
-  theorem elemFlattenAlsoElemSomeList [BEq α] [LawfulBEq α] (L : List (List α)) : ∀ e, (L.foldl (fun acc L' => acc ++ L') (List.nil)).elem e -> ∃ L', L.elem L' ∧ L'.elem e := by
+  theorem elemFlattenAlsoElemSomeList [BEq α] [LawfulBEq α] (L : List (List α)) : ∀ e, e ∈ (L.foldl (fun acc L' => acc ++ L') (List.nil)) -> ∃ L', L' ∈ L ∧ e ∈ L' := by
     intro e h_flatten
     exact elemFlattenAlsoElemSomeListHelper L e List.nil (by 
       constructor
-      . simp [elem]
+      . simp
       . exact h_flatten
     )
 
@@ -418,14 +385,12 @@ namespace List
         intro h_eq
         injection h_eq with head tail
         injection h with h
-        simp at h
         constructor
         . rw [head]
           rw [(ih cs h tail).left]
         . exact (ih cs h tail).right
 
-  theorem mapConcatEqMapParts (as bs : List α) (f : α -> β) : List.map f (as ++ bs) = as.map f ++ bs.map f := by 
-    simp
+  theorem mapConcatEqMapParts (as bs : List α) (f : α -> β) : List.map f (as ++ bs) = as.map f ++ bs.map f := by simp
 
   theorem get_eq_of_eq {as bs : List α} (h : as = bs) (idx : Fin as.length) : as.get idx = bs.get ⟨idx.val, (by rw [← h]; exact idx.isLt)⟩ := by
     cases h; rfl
