ProofLibrary/SubstitutionAndHomomorphismBasics.lean
@@ -46,7 +46,7 @@ namespace GroundSubstitution
     simp [apply_atom, List.get_map]
 
   -- TODO: is the extra assumption with injectivity reasonable?
-  theorem eq_under_subs_means_elements_are_preserved [DecidableEq SkolemTerm] (σ : GroundSubstitution) (a : Atom) (f : Fact) (h : σ.apply_atom a = f) : ∀ t, (∀ s, s ∈ a.terms.toSet ∧ σ.apply_skolem_term t = σ.apply_skolem_term s -> t = s) -> (f.terms.elem (σ.apply_skolem_term t) ↔ a.terms.elem t) := by 
+  theorem eq_under_subs_means_elements_are_preserved [DecidableEq SkolemTerm] (σ : GroundSubstitution) (a : Atom) (f : Fact) (h : σ.apply_atom a = f) : ∀ t, (∀ s, s ∈ a.terms.toSet ∧ σ.apply_skolem_term t = σ.apply_skolem_term s -> t = s) -> ((σ.apply_skolem_term t) ∈ f.terms ↔ t ∈ a.terms) := by 
     intro t ht
     rw [List.listElementIffToSetElement] 
     rw [List.listElementIffToSetElement] 
@@ -68,7 +68,7 @@ namespace GroundSubstitution
       rw [hi]
 
   -- TODO: is the extra assumption with injectivity reasonable?
-  theorem eq_under_subs_means_indices_of_elements_are_preserved [DecidableEq SkolemTerm] (σ : GroundSubstitution) (a : Atom) (f : Fact) (h : σ.apply_atom a = f) (t : SkolemTerm) (ht : a.terms.elem t) (hs : ∀ s, s ∈ a.terms.toSet ∧ σ.apply_skolem_term t = σ.apply_skolem_term s -> t = s) : (f.terms.idx_of (σ.apply_skolem_term t) (by rw [eq_under_subs_means_elements_are_preserved σ a f h t hs]; exact ht)).val = ((a.terms.idx_of t) ht).val := by 
+  theorem eq_under_subs_means_indices_of_elements_are_preserved [DecidableEq SkolemTerm] (σ : GroundSubstitution) (a : Atom) (f : Fact) (h : σ.apply_atom a = f) (t : SkolemTerm) (ht : t ∈ a.terms) (hs : ∀ s, s ∈ a.terms.toSet ∧ σ.apply_skolem_term t = σ.apply_skolem_term s -> t = s) : (f.terms.idx_of (σ.apply_skolem_term t) (by rw [eq_under_subs_means_elements_are_preserved σ a f h t hs]; exact ht)).val = ((a.terms.idx_of t) ht).val := by 
     have : f.terms = a.terms.map σ.apply_skolem_term := by rw [← h]; unfold apply_atom; simp
     rw [List.idx_of_eq_of_list_eq _ _ this _ _]
     apply Eq.symm
